\begin{align*}
e_x &= b\cos(A) + a + c\cos(A) - d\cos(B) \\
      &= a + (b + c)\cos(A) - d\cos(B) \\

e_y &= c\sin(A) - b\sin(A) - d\sin(B) \\
      &= (c - b)\sin(A) - d\sin(B) 
\\
e^2 &= e_x^2 + e_y^2 \\
    &= a^2 + (b + c)^2\cos^2(A) + d^2\cos^2(B) \\
    &\qquad + 2a(b + c)\cos(A) - 2ad\cos(B) \\
    &\qquad - 2(b + c)d\cos(A)cos(B) \\
    &\qquad + (c - b)^2\sin^2(A) + d^2\sin^2(B) \\
    &\qquad - 2(c - b)d\sin(A)\sin(B) \\
    &= a^2 - 2(b + c)d / 4 \\
    &\qquad + (b + c)^2 ( 3 - \sqrt{5}) / 8 \\
    &\qquad + d^2       ( 3 + \sqrt{5}) / 8 \\
    &\qquad + 2a(b + c) (-1 + \sqrt{5}) / 4 \\
    &\qquad - 2ad( 1 + \sqrt{5}) / 4 \\
    &\qquad + (c - b)^2 ( 5 + \sqrt{5}) / 8 \\
    &\qquad + d^2       ( 5 - \sqrt{5}) / 8 \\
    &\qquad - 2(c - b)d ( \sqrt{5}) / 4 \\
    &= m\sqrt{5} + n \\
\end{align*}