\documentclass[11pt]{article}
\title{\textbf{Meccano frames}}
\author{https://github.com/heptagons/meccano/frames}
\date{}

\usepackage{../meccano}
\usepackage{tikz}
\usetikzlibrary{calc}

\begin{document}

\maketitle
\begin{abstract}
Meccano frames are groups of meccano\meccanoref strips intended to be a
base to build diverse meccano larger objects.
\end{abstract}

\section{Triangle with extensions}

\begin{figure}[h]
\centering
\includegraphics[scale=0.75]{frame_triangle}
\caption{Triangle frame}
\label{fig:triangle}
\end{figure}



\section{Algebraic distance not right}

\begin{figure}[h]
\centering
\begin{tikzpicture}
\begin{scope}[scale=0.4]
\begin{scope}
\draw[red,dotted] (0,0) -- node[below,black]{$\sqrt{f}$}++(7,0);
\draw[black,fill=black] (7,0) node[below]{$D$}  circle(4pt)
-- node[below]{$h$} ++(5,0) node[below right]{$G$} circle(4pt)
-- node[right]{$i$} ++(-3,6) node[above]{$H$} circle(4pt)
-- node[above left]{$g-a-d$} ++(-3,-2) node[above left]{$C$} circle(4pt)
-- node[above left]{$a$} ++(-3,-2) node[above left]{$B$} circle(4pt)
-- node[above left]{$d$} ++(-3,-2) node[below left]{$E$} circle(4pt);
\draw[blue,fill=blue] (7,0)
-- node[right]{$e$} ++(-.25,1) node[above right]{$A$} circle(4pt)
-- node[right]{$b$} ++(-.75,3)
   ++(+.75,-3)
-- node[above]{$c$} (3,2);
\draw[black](6,-3) node{$(a)$};

\end{scope}

\begin{scope}[shift={(18,0)}]
\draw[red,dotted] (0,0) -- node[below,black]{$\sqrt{f}$}++(7,0);
\draw[black,fill=black] (7,0) node[below]{$D$}  circle(4pt)
-- node[below]{$h$} ++(5,0) node[below right]{$G$} circle(4pt)
-- node[right]{$i$} ++(-3,6) node[above]{$H$} circle(4pt)
-- node[above]{$g$} ++(-9,-6) node[below left]{$E$} circle(4pt);
\draw[black](6,-3) node{$(b)$};
\end{scope}


\end{scope}
\end{tikzpicture}
\caption{The five strips intented to form an algebraic distance $\sqrt{f} + h$.}
\label{fig:alg-not-right}
\end{figure}

From figure \ref{fig:alg-not-right} $(a)$ we know $\sqrt{f}$ distance
between nodes $E$ and $D$ is produced by the three strips frame $a+d$, $b+e$ and $c$.
Using the law of cosines we calculate the angle $\theta = \angle{CED}$ in terms of $\sqrt{f}$:

\begin{align}
\cos\theta &= \frac{(a+d)^2 + (\sqrt{f})^2 - (b+e)^2}{2(a+d)\sqrt{f}} \nonumber\\
 &= \frac{((a+d)^2 + f - (b+e)^2)\sqrt{f}}{2(a+d)f} \\
 &= \frac{m\sqrt{f}}{n} \label{eq:cos1}\\
 m &= (a+d)^2 + f - (b+e)^2 \\
 n &= 2(a+d)f
\end{align}

From figure \ref{fig:alg-not-right} $(a)$ we notice two sets of points are collinear:
$\{ E,B,C,H \}$ and $\{ E,D,G \}$. Using the law of cosines we calculate the 
angle $\theta = \angle{HEG}$ in terms of distances $g,h,i$:

\begin{align}
\cos\theta &= \frac{g^2 + (\sqrt{f}+h)^2 - i^2}{2g(\sqrt{f}+h)} \nonumber\\
 &= \frac{g^2 + f + 2\sqrt{f}h + h^2 - i^2}{2g(\sqrt{f}+h)} \nonumber\\
 &= \frac{g^2 + f + h^2 - i^2+ 2\sqrt{f}h}{2g(\sqrt{f}+h)}
\end{align}

We multiply both numerator and denominator by $\sqrt{f}-h$ to eliminate the surd from denominator:
\begin{align}
\cos\theta &= \frac{(f + g^2 + h^2 - i^2)(\sqrt{f}-h) + 2\sqrt{f}h(\sqrt{f}-h)}
	{2g(\sqrt{f}+h)(\sqrt{f}-h)} \nonumber\\
 &= \frac{(f + g^2 + h^2 - i^2)(\sqrt{f}-h) + 2fh - 2\sqrt{f}h^2}
	{2g(f-h^2)} \nonumber\\ 
 &= \frac{-h(f + g^2 + h^2 - i^2 - 2f) + (f + g^2 + h^2 - i^2 - 2h^2)\sqrt{f}}
	{2g(f-h^2)} \nonumber\\ 
 &= \frac{h(f - g^2 - h^2 + i^2) + (f + g^2 - h^2 - i^2)\sqrt{f}}
	{2g(f-h^2)} \nonumber\\ 
 &= \frac{o + p\sqrt{f}}{q} \label{eq:cos2}\\
o &= h(f - g^2 - h^2 + i^2) \\
p &= f + g^2 - h^2 - i^2 \\
q &= 2g(f-h^2)
\end{align}

We compare both cosines equations \ref{eq:cos1} and \ref{eq:cos2}:
\begin{align}
\frac{m\sqrt{f}}{n} &= \frac{o + p\sqrt{f}}{q}
\end{align}
Since all variables are integers we need two conditions. First $o$ should be zero.
And second $\frac{m}{n} = \frac{p}{q}$.

For condition 1, we force $o$ to be zero:
\begin{align}
o &= 0 \nonumber\\
h(f - g^2 - h^2 + i^2) & = 0 \nonumber\\
f &= g^2 + h^2 - i^2 \label{eq:condition1}
\end{align}

For condition2, we force $m,n,p,q$ as:
\begin{align}
\frac{m}{n} &= \frac{p}{q} \nonumber\\
\frac{(a+d)^2 + f - (b+e)^2}{2(a+d)f} &= \frac{f + g^2 - h^2 - i^2}{2g(f-h^2)} \nonumber\\
\end{align}

We replace the value of $f$ of last equation RHS with the value of equation \ref{eq:condition1}
of condition 1:
\begin{align}
\frac{(a+d)^2 - (b+e)^2 + f}{(a+d)f} &= \frac{f + g^2 - h^2 - i^2}{g(f-h^2)} \nonumber\\
 &= \frac{g^2 + h^2 - i^2 + g^2 - h^2 - i^2}{g(g^2 + h^2 - i^2-h^2)} \nonumber\\
 &= \frac{2(g^2 - i^2)}{g(g^2 - i^2)} \nonumber\\
 &= \frac{2}{g} \nonumber\\
((a+d)^2 - (b+e)^2 + f)g &= 2(a+d)f \label{eq:condition2}
\end{align}















\end{document}